src/Data/Monoid.v
@@ -5,17 +5,23 @@ Set Primitive Projections.
 
 Class Monoid (m : Type) := {
   is_semigroup :> Semigroup m;
-
   mempty : m;
-
-  mempty_left  : forall a, mappend mempty a = a;
-  mempty_right : forall a, mappend a mempty = a;
 }.
 
 #[global]
 Program Instance Monoid_option `{Monoid a} : Monoid (option a) := {
   mempty := None
 }.
+
+Class MonoidLaws (m : Type) `{Monoid m} := {
+  has_semigroup_laws :> SemigroupLaws m;
+
+  mempty_left  : forall a, mappend mempty a = a;
+  mempty_right : forall a, mappend a mempty = a;
+}.
+
+#[global]
+Program Instance MonoidLaws_option `{MonoidLaws a} : MonoidLaws (option a).
 Next Obligation.
   destruct a0; reflexivity.
 Qed.
